Sodium/Ethos/Server.lean
@@ -1,0 +1,83 @@
+import Sodium.Ethos.Frontend
+import Lean.Server.Requests
+
+universe u
+
+open Lean Sodium Server Crypto
+
+namespace Ethos.Server
+
+deriving instance TypeName for Meta.SavedState
+
+structure EthosRequest where
+  text : Lsp.TextDocumentIdentifier
+  position : Lsp.Position
+  cert : Observable
+
+instance : Lsp.FileSource EthosRequest where
+  fileSource p := p.text.uri
+
+instance _root_.Lsp.TextDocumentIdentifier.encodable : Encodable Lsp.TextDocumentIdentifier :=
+  Encodable.ofEquiv _ {
+    push x := x.uri
+    pull x := ⟨x⟩
+  }
+
+instance _root_.Lsp.Position.encodable : Encodable Lsp.Position :=
+  Encodable.ofEquiv (Nat × Nat) {
+    push | ⟨x, y⟩ => ⟨x, y⟩
+    pull | ⟨x, y⟩ => ⟨x, y⟩
+  }
+
+def EthosRequest.Shape :=
+  Lsp.TextDocumentIdentifier
+  × Lsp.Position
+  × Observable
+
+instance EthosRequest.Shape.encodable : Encodable EthosRequest.Shape := by unfold Shape; infer_instance
+
+instance EthosRequest.encodable : Encodable EthosRequest :=
+  Encodable.ofEquiv Shape {
+    push | ⟨x₁, x₂, x₃⟩ => ⟨x₁, x₂, x₃⟩
+    pull | ⟨x₁, x₂, x₃⟩ => ⟨x₁, x₂, x₃⟩
+  }
+
+instance : ToJson Observable := ⟨encode⟩
+instance : FromJson EthosRequest := ⟨fun x => match decode? x with | some x => .ok x | _ => .error s!"{decl_name%}"⟩
+
+protected def main (p : EthosRequest) (ctx : Meta.SavedState) : RequestM (LspResponse Observable × Meta.SavedState) := do
+  let ε : {σ : Type} → (τ : Sodium σ) → EthosM τ Observable := fun τ => by
+    ethos addressed (prompt := default) (add norm unfold Ethos.Universal.prompt) fun msg => do
+      unless this.phase = .safe do default
+      let .accepted o ← decrypt? (α := Observable) msg | default
+      o.quantize
+
+  let main : MetaM Observable := do
+    let δ ← mkFreshDelta
+    let o? ← Ethos.main ε δ.mvarId!
+    return o?.get
+
+  let o? ← RequestM.withWaitFindSnapAtPos p.position fun snap => do RequestM.runCoreM snap fun _ => do
+    let ⟨⟨o, stale⟩, fresh⟩ ← ctx.runMetaM main |>.run
+    return ⟨⟨o, true⟩, {stale with meta := fresh}⟩
+
+  return match o?.get with
+  | .ok x => x
+  | .error s => ⟨⟨p.cert, false⟩, ctx⟩
+
+protected def turn (e : Lsp.DidChangeTextDocumentParams) : StateT Meta.SavedState RequestM Unit := do
+  default
+
+initialize do
+  registerPartialStatefulLspRequestHandler
+    (method := "$/lean/ethos/observe")
+    (refreshMethod := "$/lean/ethos/renew")
+    (refreshIntervalMs := 1000)
+    (paramType := EthosRequest)
+    (respType := Observable)
+    (stateType := Meta.SavedState)
+    (initState := {core := {env := ← mkEmptyEnvironment, passedHeartbeats := ← IO.getNumHeartbeats}, meta := {}})
+    Ethos.Server.main
+    Ethos.Server.turn
+
+end Ethos.Server
