Sodium/Polybius/Basic.lean
@@ -1,1 +1,11 @@
 import Sodium.Ethos
+
+open Lean Elab Sodium
+
+/-
+Polybius is a secure, distributed, interactive theorem proving system.
+-/
+
+namespace Polybius
+
+end Polybius
